devel/Iron/SystemF2Effect/Store/StoreM.v
@@ -1,0 +1,27 @@
+
+Require Export Iron.SystemF2Effect.Step.Frame.
+Require Export Iron.SystemF2Effect.Store.Bind.
+
+
+(* Store typing models the store.
+   All types in the store typing have a corresponding binding in the store.
+   We don't want entries in the store typing that don't have corresponding
+   bindings in the store. *)
+
+Definition STOREM (se: stenv) (ss: store)
+ := length se = length ss.
+Hint Unfold STOREM.
+
+
+(* Extended store environment models the extended store *)
+Lemma storem_snoc
+ :  forall se ss t stv
+ ,  STOREM se ss
+ -> STOREM (t <: se) (stv <: ss).
+Proof.
+ intros.
+ unfold STOREM.
+ have (length se = length ss). 
+ burn.
+Qed.
+Hint Resolve storem_snoc.
